

$$\begin{aligned}
V_{1,1} &= \bigwedge_{i=1}^3 V_{1i,1} \\
V_{1,2} &= \left(V_{1,1} \wedge \left(\bigwedge_{i=1}^3 V_{1i,1} \right) \right) \vee \left(\neg V_{1,1} \wedge \left(\bigwedge_{i=1}^3 (V_{1i,1} \vee V_{1i,2}) \right) \right) \\
V_{1,3} &= \left(V_{1,1} \wedge V_{1,2} \wedge \left(\bigwedge_{i=1}^3 V_{1i,3} \right) \right) \vee \left(V_{1,1} \wedge \neg V_{1,2} \wedge \left(\bigwedge_{i=1}^3 (V_{1i,2} \vee V_{1i,3}) \right) \right) \vee \\
&\quad \left(\neg V_{1,1} \wedge V_{1,2} \wedge \left(\bigwedge_{i=1}^3 (V_{1i,1} \vee \neg V_{1i,2} \vee V_{1i,3}) \right) \right) \vee \left(\neg V_{1,1} \wedge \neg V_{1,2} \wedge \left(\bigwedge_{i=1}^3 (V_{1i,1} \vee V_{1i,2} \vee V_{1i,3}) \right) \right) \\
&\text{Simplifies to:} \\
V_{1,1} &= \bigwedge_{i=1}^3 V_{1i,1} \\
V_{1,2} &= \bigwedge_{i=1}^3 (V_{1i,2} \vee (V_{1i,1} \oplus V_{1,1})) \\
V_{1,3} &= \bigwedge_{i=1}^3 (V_{1i,3} \vee (V_{1i,2} \oplus V_{1,2}) \vee (V_{1i,1} \oplus V_{1,1}))
\end{aligned}$$